Cleanup of RBT.

HOL/DataStrs/RBT_Base.thy
@@ -10,7 +10,7 @@ theory RBT_Base
 imports Lists_Ex
 begin
 
-section {* Definition of RBT, and basic setup *}
+section {* Definition of RBT *}
 
 datatype color = R | B
 datatype ('a, 'b) pre_rbt =
@@ -26,92 +26,72 @@ setup {* add_forward_prfstep (equiv_forward_th (@{thm pre_rbt.simps(1)})) *}
 setup {* add_forward_prfstep @{thm pre_rbt.collapse} *}
 setup {* add_var_induct_rule @{thm pre_rbt.induct} *}
 
-subsection {* Some trivial lemmas *}
+lemma not_R [forward]: "c \<noteq> R \<Longrightarrow> c = B" using color.exhaust by blast
+lemma not_B [forward]: "c \<noteq> B \<Longrightarrow> c = R" using color.exhaust by blast
+lemma red_not_leaf [forward]: "cl t = R \<Longrightarrow> t \<noteq> Leaf" by auto
 
-theorem not_R [forward]: "c \<noteq> R \<Longrightarrow> c = B" using color.exhaust by blast
-theorem not_B [forward]: "c \<noteq> B \<Longrightarrow> c = R" using color.exhaust by blast
-theorem red_not_leaf [forward]: "cl t = R \<Longrightarrow> t \<noteq> Leaf" by auto
-
-section {* Definition of main functions and invariants *}
-
-fun min_depth :: "('a, 'b) pre_rbt \<Rightarrow> nat" where
-  "min_depth Leaf = 0"
-| "min_depth (Node l c k v r) = min (min_depth l) (min_depth r) + 1"
-
-fun max_depth :: "('a, 'b) pre_rbt \<Rightarrow> nat" where
-  "max_depth Leaf = 0"
-| "max_depth (Node l c k v r) = max (max_depth l) (max_depth r) + 1"
+section {* RBT invariants *}
 
 fun black_depth :: "('a, 'b) pre_rbt \<Rightarrow> nat" where
   "black_depth Leaf = 0"
 | "black_depth (Node l R k v r) = black_depth l"
 | "black_depth (Node l B k v r) = black_depth l + 1"
+setup {* fold add_rewrite_rule @{thms black_depth.simps} *}
 
 fun cl_inv :: "('a, 'b) pre_rbt \<Rightarrow> bool" where
   "cl_inv Leaf = True"
 | "cl_inv (Node l R k v r) = (cl_inv l \<and> cl_inv r \<and> cl l = B \<and> cl r = B)"
 | "cl_inv (Node l B k v r) = (cl_inv l \<and> cl_inv r)"
+setup {* fold add_rewrite_rule @{thms cl_inv.simps} *}
 setup {* add_property_const @{term cl_inv} *}
 
 fun bd_inv :: "('a, 'b) pre_rbt \<Rightarrow> bool" where
   "bd_inv Leaf = True"
 | "bd_inv (Node l c k v r) = (bd_inv l \<and> bd_inv r \<and> black_depth l = black_depth r)"
+setup {* fold add_rewrite_rule @{thms bd_inv.simps} *}
 setup {* add_property_const @{term bd_inv} *}
 
-definition is_rbt :: "('a, 'b) pre_rbt \<Rightarrow> bool" where
+definition is_rbt :: "('a, 'b) pre_rbt \<Rightarrow> bool" where [rewrite]:
   "is_rbt t = (cl_inv t \<and> bd_inv t)"
 setup {* add_property_const @{term is_rbt} *}
-
-setup {* fold add_rewrite_rule (
-  @{thms min_depth.simps} @ @{thms max_depth.simps} @ @{thms black_depth.simps} @
-  @{thms cl_inv.simps} @ @{thms bd_inv.simps} @ [@{thm is_rbt_def}]) *}
 
 lemma cl_invI: "cl_inv l \<Longrightarrow> cl_inv r \<Longrightarrow> cl_inv (Node l B k v r)" by auto2
 setup {* add_forward_prfstep_cond @{thm cl_invI} [with_term "Node ?l B ?k ?v ?r"] *}
 
-subsection {* Properties of bd_inv *}
+lemma bd_invI: "bd_inv l \<Longrightarrow> bd_inv r \<Longrightarrow> black_depth l = black_depth r \<Longrightarrow> bd_inv (Node l c k v r)" by auto2
+setup {* add_forward_prfstep_cond @{thm bd_invI} [with_term "Node ?l ?c ?k ?v ?r"] *}
 
-lemma bd_inv_intro:
-  "bd_inv l \<Longrightarrow> bd_inv r \<Longrightarrow> black_depth l = black_depth r \<Longrightarrow> bd_inv (Node l c k v r)" by auto2
-setup {* add_forward_prfstep_cond @{thm bd_inv_intro} [with_term "Node ?l ?c ?k ?v ?r"] *}
-
-subsection {* is_rbt is recursive *}
-
-theorem is_rbt_rec [forward]: "is_rbt (Node l c k v r) \<Longrightarrow> is_rbt l \<and> is_rbt r"
+lemma is_rbt_rec [forward]: "is_rbt (Node l c k v r) \<Longrightarrow> is_rbt l \<and> is_rbt r"
 @proof @case "c = R" @qed
 
-section {* Balancedness of is_rbt *}
+section {* Balancedness of RBT *}
 
-theorem depth_min: "is_rbt t \<Longrightarrow> black_depth t \<le> min_depth t"
+(* Remove after having general normalization procedure for nats. *)
+lemma two_distrib [rewrite]: "(2::nat) * (a + 1) = 2 * a + 2" by simp
+
+fun min_depth :: "('a, 'b) pre_rbt \<Rightarrow> nat" where
+  "min_depth Leaf = 0"
+| "min_depth (Node l c k v r) = min (min_depth l) (min_depth r) + 1"
+setup {* fold add_rewrite_rule @{thms min_depth.simps} *}
+
+fun max_depth :: "('a, 'b) pre_rbt \<Rightarrow> nat" where
+  "max_depth Leaf = 0"
+| "max_depth (Node l c k v r) = max (max_depth l) (max_depth r) + 1"
+setup {* fold add_rewrite_rule @{thms max_depth.simps} *}
+
+theorem rbt_balanced: "is_rbt t \<Longrightarrow> max_depth t \<le> 2 * min_depth t + 1"
 @proof
-  @induct t @with
-    @subgoal "t = Node l c k v r"
-      @case "c = R" @with
-      @have "black_depth (Node l c k v r) \<le> min (min_depth l) (min_depth r)" @end
-    @endgoal
+  @induct t for "is_rbt t \<longrightarrow> black_depth t \<le> min_depth t" @with
+    @subgoal "t = Node l c k v r" @case "c = R" @endgoal
   @end
+  @induct t for "is_rbt t \<longrightarrow> (if cl t = R then max_depth t \<le> 2 * black_depth t + 1
+                               else max_depth t \<le> 2 * black_depth t)" @with
+    @subgoal "t = Node l c k v r" @case "c = R" @endgoal
+  @end
+  @have "max_depth t \<le> 2 * black_depth t + 1"
 @qed
 
-theorem two_distrib [rewrite]: "(2::nat) * (a + 1) = 2 * a + 2" by simp
-theorem depth_max: "is_rbt t \<Longrightarrow> if cl t = R then max_depth t \<le> 2 * black_depth t + 1
-                                 else max_depth t \<le> 2 * black_depth t"
-@proof
-  @induct t @with
-    @subgoal "t = Node l c k v r"
-      @case "c = R" @then
-      @have "max_depth l \<le> 2 * black_depth l + 1" @then
-      @have "max_depth r \<le> 2 * black_depth r + 1"
-    @endgoal
-  @end
-@qed
-
-setup {* fold add_forward_prfstep [@{thm depth_min}, @{thm depth_max}] *}
-
-theorem balanced: "is_rbt t \<Longrightarrow> max_depth t \<le> 2 * min_depth t + 1"
-@proof @have "max_depth t \<le> 2 * black_depth t + 1" @qed
-setup {* fold del_prfstep_thm [@{thm depth_min}, @{thm depth_max}] *}
-
-subsection {* Definition and basic properties of cl_inv' *}
+section {* Definition and basic properties of cl_inv' *}
 
 fun cl_inv' :: "('a, 'b) pre_rbt \<Rightarrow> bool" where
   "cl_inv' Leaf = True"
@@ -119,18 +99,18 @@ fun cl_inv' :: "('a, 'b) pre_rbt \<Rightarrow> bool" where
 setup {* fold add_rewrite_rule @{thms cl_inv'.simps} *}
 setup {* add_property_const @{term cl_inv'} *}
 
-theorem cl_inv_B [forward, backward1]:
+lemma cl_inv'B [forward, backward1]:
   "cl_inv' t \<Longrightarrow> cl t = B \<Longrightarrow> cl_inv t"
 @proof @case "t = Leaf" @qed
 
-theorem cl_inv_R [forward]:
+lemma cl_inv'R [forward]:
   "cl_inv' (Node l R k v r) \<Longrightarrow> cl l = B \<Longrightarrow> cl r = B \<Longrightarrow> cl_inv (Node l R k v r)" by auto2
 
-theorem cl_inv_imp [forward]: "cl_inv t \<Longrightarrow> cl_inv' t"
+lemma cl_inv_to_cl_inv' [forward]: "cl_inv t \<Longrightarrow> cl_inv' t"
 @proof @case "t = Leaf" @then @case "cl t = R" @qed
 
-theorem cl_inv'I: "cl_inv l \<Longrightarrow> cl_inv r \<Longrightarrow> cl_inv' (Node l c k v r)" by auto
-setup {* add_forward_prfstep_cond @{thm cl_inv'I} [with_term "cl_inv' (Node ?l ?c ?k ?v ?r)"] *}
+lemma cl_inv'I: "cl_inv l \<Longrightarrow> cl_inv r \<Longrightarrow> cl_inv' (Node l c k v r)" by auto
+setup {* add_forward_prfstep_cond @{thm cl_inv'I} [with_term "Node ?l ?c ?k ?v ?r"] *}
 
 subsection {* Set of keys, sortedness *}
 
@@ -149,10 +129,8 @@ fun rbt_in_traverse_pairs :: "('a, 'b) pre_rbt \<Rightarrow> ('a \<times> 'b) li
 | "rbt_in_traverse_pairs (Node l c k v r) = (rbt_in_traverse_pairs l) @ [(k, v)] @ (rbt_in_traverse_pairs r)"
 setup {* fold add_rewrite_rule @{thms rbt_in_traverse_pairs.simps} *}
 
-theorem rbt_in_traverse_fst:
-  "map fst (rbt_in_traverse_pairs t) = rbt_in_traverse t"
+lemma rbt_in_traverse_fst [rewrite]: "map fst (rbt_in_traverse_pairs t) = rbt_in_traverse t"
 @proof @induct t @qed
-setup {* add_forward_prfstep_cond @{thm rbt_in_traverse_fst} [with_term "rbt_in_traverse_pairs ?t"] *}
 
 definition rbt_map :: "('a, 'b) pre_rbt \<Rightarrow> ('a, 'b) map" where
   "rbt_map t = map_of_alist (rbt_in_traverse_pairs t)"
@@ -160,19 +138,19 @@ setup {* add_rewrite_rule @{thm rbt_map_def} *}
 
 fun rbt_sorted :: "('a::linorder, 'b) pre_rbt \<Rightarrow> bool" where
   "rbt_sorted Leaf = True"
-| "rbt_sorted (Node l c k v r) = ((\<forall>x\<in>rbt_set l. x < k) \<and> (\<forall>x\<in>rbt_set r. k < x)
-                                  \<and> rbt_sorted l \<and> rbt_sorted r)"
+| "rbt_sorted (Node l c k v r) = ((\<forall>x\<in>rbt_set l. x < k) \<and> (\<forall>x\<in>rbt_set r. k < x) \<and> rbt_sorted l \<and> rbt_sorted r)"
 setup {* fold add_rewrite_rule @{thms rbt_sorted.simps} *}
+setup {* add_property_const @{term rbt_sorted} *}
 
-theorem rbt_sorted_lr [forward]:
+lemma rbt_sorted_lr [forward]:
   "rbt_sorted (Node l c k v r) \<Longrightarrow> rbt_sorted l \<and> rbt_sorted r" by auto2
 
-theorem rbt_inorder_preserve_set [rewrite_back]:
-  "set (rbt_in_traverse t) = rbt_set t"
+lemma rbt_inorder_preserve_set [rewrite]:
+  "rbt_set t = set (rbt_in_traverse t)"
 @proof @induct t @qed
 
-theorem rbt_inorder_sorted [rewrite_back]:
-  "strict_sorted (rbt_in_traverse t) = rbt_sorted t"
+lemma rbt_inorder_sorted [rewrite]:
+  "rbt_sorted t \<longleftrightarrow> strict_sorted (map fst (rbt_in_traverse_pairs t))"
 @proof @induct t @qed
 
 setup {* fold del_prfstep_thm (@{thms rbt_set.simps} @ @{thms rbt_sorted.simps}) *}
